common/dnf.lean
@@ -2,7 +2,7 @@ import .atom
 
 variables {α β : Type}
 
-open atom_type
+open atom_type list
 
 /-
 Requires : nqfree arg-0
@@ -11,35 +11,37 @@ def dnf : fm α → list (list α)
 | (fm.true α) := [[]]
 | (fm.false α) := []
 | (fm.atom a) := [[a]]
-| (fm.and p q) := list.map append_pair $ list.product (dnf p) (dnf q)
+| (fm.and p q) := list.map list.append_pair $ list.product (dnf p) (dnf q)
 | (fm.or p q) := dnf p ++ dnf q 
 | (fm.ex _) := []
 | (fm.not _) := []
 
 lemma dnf_prsv_pred [atom_type α β] (pr : α → Prop) : 
-  ∀ (φ : fm α), allp pr (@atoms _ (atom_type.dec_eq _ β) φ) → allp (allp pr) (dnf φ) 
+  ∀ (φ : fm α), list.allp pr (@atoms _ (atom_type.dec_eq _ β) φ) → list.allp (list.allp pr) (dnf φ) 
 | (fm.true α) hnm := 
   begin
-    intros as has, unfold dnf at has,
-    rewrite exp_mem_singleton at has, subst has,
-    apply allp_nil
+    intros as has, unfold dnf at has, simp,
+    rewrite list.mem_singleton at has, subst has,
+    apply list.forall_mem_nil
   end
-| (fm.false α) hnm := allp_nil
+| (fm.false α) hnm := 
+  begin simp, unfold dnf, intros a ha, cases ha end
 | (fm.atom a) hnm := 
   begin
     intros as has, unfold dnf at has,
-    rewrite exp_mem_singleton at has, 
+    rewrite mem_singleton at has, 
     subst has, intros a' ha', 
-    rewrite exp_mem_singleton at ha',
+    rewrite mem_singleton at ha',
     subst ha', apply hnm, apply or.inl rfl
   end
 | (fm.and p q) hnm := 
   begin 
-    unfold atoms at hnm,
-    rewrite exp_allp_union at hnm,
+    unfold atoms at hnm, 
+    rewrite allp_iff_forall_mem at hnm,
+    rewrite forall_mem_union at hnm,
     cases hnm with hnmp hnmq,
     unfold dnf, intros as has, intros a ha,
-    rewrite exp_mem_map at has, 
+    rewrite mem_map at has, 
     cases has with asp hasp, 
     cases hasp with hasp1 hasp2,
     cases asp with as1 as2, subst hasp2, 
@@ -52,38 +54,45 @@ lemma dnf_prsv_pred [atom_type α β] (pr : α → Prop) :
 | (fm.or p q) hnm := 
   begin
     unfold atoms at hnm, 
-    rewrite exp_allp_union at hnm,
+    rewrite allp_iff_forall_mem at hnm,
+    rewrite forall_mem_union at hnm,
     cases hnm with hnmp hnmq,
     unfold dnf, intros as has, intros a ha,
     cases (mem_or_mem_of_mem_append has) with hm hm,
     apply dnf_prsv_pred p hnmp as hm a ha, 
     apply dnf_prsv_pred q hnmq as hm a ha 
   end
-| (fm.not _) hnm := allp_nil
-| (fm.ex _) hnm := allp_nil
-
+| (fm.not _) hnm := 
+  begin
+    rewrite allp_iff_forall_mem, 
+    unfold dnf, apply @forall_mem_nil _ (allp pr),
+  end
+| (fm.ex _) hnm := 
+  begin
+    rewrite allp_iff_forall_mem, 
+    unfold dnf, apply @forall_mem_nil _ (allp pr),
+  end
+  
 lemma dnf_prsv_normal [atom_type α β] : ∀ (p : fm α), 
-  fnormal β p → allp (allp (normal β)) (dnf p) := 
+  fnormal β p → list.allp (list.allp (normal β)) (dnf p) := 
 begin
   intros p hp, rewrite fnormal_iff_fnormal_alt at hp,
   apply dnf_prsv_pred (normal β) _ hp, 
 end
 
+#check @mem_map_of_mem
 lemma dnf_prsv_alt [atom_type α β] : ∀ {p : fm α} {H : nqfree p} {xs : list β}, 
-  disj_list (list.map (allp (atom_type.val xs)) (dnf p)) ↔ I p xs 
+  list.disj_list (list.map (allp (atom_type.val xs)) (dnf p)) ↔ I p xs 
 | (fm.true α) H bs := 
   by {unfold dnf, simp, unfold disj_list, 
-      rewrite exp_allp_nil, rewrite true_or,
-      unfold I, unfold interp}
+      rewrite true_or, unfold I, unfold interp}
 | (fm.false α) H bs := 
   by {unfold dnf, simp, unfold disj_list, rewrite exp_I_bot }
 | (fm.atom a) H bs := 
   begin
     unfold dnf, simp, unfold disj_list, simp, 
     apply iff.intro, intro Ha, apply Ha, 
-    apply or.inl rfl, intros Ha a' Ha', 
-    rewrite exp_mem_singleton at Ha', subst Ha',
-    apply Ha
+    unfold I, unfold interp, apply id
   end
 | (fm.and p q) H bs := 
   begin
@@ -97,22 +106,29 @@ lemma dnf_prsv_alt [atom_type α β] : ∀ {p : fm α} {H : nqfree p} {xs : list
     intro H0, cases H0 with r Hr, 
     have Hrl := Hr^.elim_left,
     have Hrr := Hr^.elim_right, clear Hr, 
-    cases (ex_arg_of_mem_map Hrl) with d Hd,
+    cases (list.exists_of_mem_map Hrl) with d Hd,
     simp at Hd, 
     apply and.intro, 
          
     existsi (∀ (a : α), a ∈ (prod.fst d) → atom_type.val bs a),
-    apply and.intro, apply mem_map_of_mem,
-    apply fst_mem_of_mem_product Hd^.elim_right,
-    intros a Ha, rewrite Hd^.elim_left at Hrr,
+    cases Hd with hd1 hd2,
+    apply and.intro, 
+    rewrite iff.symm (allp_iff_forall_mem (val bs) d.fst), 
+    apply mem_map_of_mem,
+    
+    apply fst_mem_of_mem_product, apply hd1,
+    intros a Ha, subst hd2,
     apply Hrr, cases d with dl dr, unfold append_pair,
     apply mem_append_of_mem_or_mem,
     apply or.inl Ha, 
 
     existsi (∀ (a : α), a ∈ (prod.snd d) → atom_type.val bs a),
-    apply and.intro, apply mem_map_of_mem, 
-    apply snd_mem_of_mem_product Hd^.elim_right,
-    intros a Ha, rewrite Hd^.elim_left at Hrr,
+    cases Hd with hd1 hd2,
+    apply and.intro, 
+    rewrite iff.symm (allp_iff_forall_mem (val bs) d.snd), 
+    apply mem_map_of_mem, 
+    apply snd_mem_of_mem_product hd1,
+    intros a Ha, subst hd2,
     apply Hrr, cases d with dl dr, unfold append_pair,
     apply mem_append_of_mem_or_mem,
     apply or.inr Ha, 
@@ -120,11 +136,13 @@ lemma dnf_prsv_alt [atom_type α β] : ∀ {p : fm α} {H : nqfree p} {xs : list
     intro H0, 
     cases (H0^.elim_left) with r Hr,
     cases (H0^.elim_right) with s Hs, clear H0, 
-    cases (ex_arg_of_mem_map Hr^.elim_left) with ll Hll,
-    cases (ex_arg_of_mem_map Hs^.elim_left) with lr Hlr,
+    cases (list.exists_of_mem_map Hr^.elim_left) with ll Hll,
+    cases (list.exists_of_mem_map Hs^.elim_left) with lr Hlr,
     existsi (∀ (a : α), a ∈ append_pair (ll,lr) → atom_type.val bs a),
-    apply and.intro, apply mem_map_of_mem, 
-    apply mem_product_of_mem_of_mem,
+    apply and.intro, 
+    rewrite iff.symm (allp_iff_forall_mem (val bs) (append_pair (ll,lr))),
+    apply mem_map_of_mem _, 
+    apply mem_product_of_mem_and_mem,
     apply Hll^.elim_left, apply Hlr^.elim_left,
     intros a Ha, 
     cases (mem_or_mem_of_mem_append Ha) with HM HM,
@@ -136,7 +154,7 @@ lemma dnf_prsv_alt [atom_type α β] : ∀ {p : fm α} {H : nqfree p} {xs : list
   end
 | (fm.or p q) H bs := 
   begin
-    unfold dnf, rewrite map_dist_append, 
+    unfold dnf, rewrite map_append, 
     rewrite disj_list_dist_append,
     rewrite dnf_prsv_alt, rewrite dnf_prsv_alt,
     rewrite exp_I_or, apply H^.elim_right,
@@ -146,5 +164,5 @@ lemma dnf_prsv_alt [atom_type α β] : ∀ {p : fm α} {H : nqfree p} {xs : list
 | (fm.ex p) H bs := by cases H
 
 lemma dnf_prsv [atom_type α β] {p : fm α} {H : nqfree p} {bs : list β} : 
-  some_true (list.map (allp (atom_type.val bs)) (dnf p)) ↔ I p bs := 
+  list.some_true (list.map (allp (atom_type.val bs)) (dnf p)) ↔ I p bs := 
 iff.trans (by rewrite some_true_iff_disj_list) (@dnf_prsv_alt _ _ _ _ H _)
