common/list.lean
@@ -1,20 +1,21 @@
-import .auxiliary
+import .auxiliary ...mathlib.data.list.basic
 
 variables {α β γ : Type}
 
-def list.sum [has_zero α] [has_add α] : list α → α 
-| [] := @has_zero.zero α _
-| (a::as) := a + list.sum as
+namespace list
+-- def list.sum [has_zero α] [has_add α] : list α → α 
+-- | [] := @has_zero.zero α _
+-- | (a::as) := a + list.sum as
 
-def list.zip_pad (a' b') : list α → list β → list (α × β)
+def zip_pad (a' b') : list α → list β → list (α × β)
 | [] [] := []
-| [] (b::bs) := (a',b)::(list.zip_pad [] bs)
-| (a::as) [] := (a,b')::(list.zip_pad as [])
-| (a::as) (b::bs) := (a,b)::(list.zip_pad as bs)
+| [] (b::bs) := (a',b)::(zip_pad [] bs)
+| (a::as) [] := (a,b')::(zip_pad as [])
+| (a::as) (b::bs) := (a,b)::(zip_pad as bs)
 
-lemma exp_zip {a b a' b'} {as : list α} {bs : list β} : 
-  list.zip_pad a' b' (a::as) (b::bs) = (a,b)::(list.zip_pad a' b' as bs) :=
-begin unfold list.zip_pad end
+lemma cons_zip_pad_cons {a b a' b'} {as : list α} {bs : list β} : 
+  zip_pad a' b' (a::as) (b::bs) = (a,b)::(zip_pad a' b' as bs) :=
+begin unfold zip_pad end
 
 def map_mul [has_mul α] (a) (as : list α) : list α :=
 list.map (λ x, a * x) as
@@ -25,47 +26,33 @@ list.map (λ xy, prod.fst xy + prod.snd xy) (list.zip_pad 0 0 as1 as2)
 def dot_prod [has_zero α] [has_add α] [has_mul α] (as1 as2 : list α) : α := 
 list.sum (list.map (λ xy, prod.fst xy * prod.snd xy) (list.zip_pad 0 0 as1 as2))
 
--- lemma dot_prod_nil_cons [has_zero α] [has_add α] [has_mul α] (a) (as : list α) :
-  -- dot_prod [] (a::as) = (0 * a) + (dot_prod [] as) := 
--- begin
-  -- unfold dot_prod, unfold list.zip_pad, 
-  -- simp, unfold list.sum, 
--- end
-
 lemma nil_dot_prod [semiring α] :
   ∀ (as : list α), dot_prod [] as = 0  
 | [] := 
   begin
-    unfold dot_prod, unfold list.zip_pad, 
-    simp, unfold list.sum
+    unfold dot_prod, unfold list.zip_pad, simp
   end
 | (a::as) := 
   begin
     unfold dot_prod, unfold list.zip_pad,
-    simp, unfold list.sum, rewrite zero_add,
-    apply nil_dot_prod
+    simp, apply nil_dot_prod
   end
 
 lemma dot_prod_nil [semiring α] :
   ∀ (as : list α), dot_prod as [] = 0  
 | [] := 
   begin
-    unfold dot_prod, unfold list.zip_pad, 
-    simp, unfold list.sum
+    unfold dot_prod, unfold list.zip_pad, simp
   end
 | (a::as) := 
   begin
     unfold dot_prod, unfold list.zip_pad,
-    simp, unfold list.sum, rewrite zero_add,
-    apply dot_prod_nil
+    simp, apply dot_prod_nil
   end
 
-lemma cons_dot_prod_cons [has_zero α] [has_add α] [has_mul α] (a1 a2 : α) (as1 as2 : list α) : 
+lemma cons_dot_prod_cons [semiring α] (a1 a2 : α) (as1 as2 : list α) : 
 dot_prod (a1::as1) (a2::as2) = (a1 * a2) + dot_prod as1 as2 := 
-begin
-  unfold dot_prod, rewrite exp_zip,
-  simp, unfold list.sum
-end
+begin unfold dot_prod, rewrite cons_zip_pad_cons, simp end
 
 lemma nil_comp_add [semiring α] :
   ∀ (as : list α), comp_add [] as = as 
@@ -131,10 +118,10 @@ lemma map_mul_dot_prod [semiring α] (a : α) :
   begin
     unfold map_mul, simp, repeat {rewrite cons_dot_prod_cons}, 
     have h := map_mul_dot_prod as1 as2, unfold map_mul at h, 
-    rewrite h, rewrite mul_add, simp,
+    rewrite h, rewrite mul_add, simp, rewrite mul_assoc
   end
 
-def exp_neg_dot_prod [ring α] : ∀ (as1 as2 : list α),  
+def neg_dot_prod [ring α] : ∀ (as1 as2 : list α),  
   dot_prod (list.map (λ x, -x) as1) as2 = -(dot_prod as1 as2) := 
 begin
   intros as1 as2,
@@ -142,32 +129,69 @@ begin
   unfold map_mul at h, simp at h, simp, apply h
 end
 
-def list.omap (f : α → option β) : list α → list β  
+/- omap -/
+
+def omap (f : α → option β) : list α → list β  
 | [] := []
 | (a::as) := 
   match f a with 
-  | none := list.omap as 
-  | (some b) := b::(list.omap as) 
+  | none := omap as 
+  | (some b) := b::(omap as) 
   end
 
-lemma exp_mem_cons {a' a : α} {as} : a' ∈ a::as ↔ (a' = a ∨ a' ∈ as) := 
-by {unfold has_mem.mem, unfold list.mem}
+lemma mem_omap {f : α → option β} {a} {b} (he : f a = some b) : 
+  ∀ {as : list α} (HM : a ∈ as), b ∈ omap f as  
+| [] hm := by cases hm
+| (a'::as) hm :=
+  begin 
+    unfold has_mem.mem at hm, unfold list.mem at hm,
+    cases hm with hm hm, subst hm,
+    unfold omap, rewrite he, apply or.inl rfl,
+    unfold omap, cases (f a'), 
+    apply mem_omap, apply hm, 
+    apply or.inr, apply mem_omap, apply hm 
+  end 
 
-lemma exp_mem_nil {a : α} : (a ∈ ([] : list α)) ↔ false := 
+lemma mem_omap_of_mem_omap_tail {f : α → option β} {a} {b} :
+  ∀ {as : list α}, b ∈ omap f as → b ∈ omap f (a::as) := 
 begin
-  apply iff.intro; intro h, cases h, 
-  exfalso, apply h
+  intros as h, unfold omap, cases (f a),
+  apply h, apply or.inr h
 end
 
-lemma exp_mem_singleton {a' a : α} : a' ∈ [a] ↔ (a' = a) := 
-begin
-  rewrite exp_mem_cons, rewrite exp_mem_nil,  
-  rewrite or_false
-end
-
-lemma eq_nil_of_map_eq_nil {f : α → β} {as}  
-  (h : list.map f as = []) : as = [] :=
-begin cases as, refl, cases h end
+lemma exp_mem_omap {f : α → option β} {b : β} : ∀ {as : list α}, (b ∈ omap f as) ↔ ∃ a, a ∈ as ∧ some b = f a 
+| [] := 
+  iff.intro 
+    (by {intro h, cases h}) 
+    (begin intro h, cases h with a ha, cases ha^.elim_left end)
+| (a::as) := 
+ iff.intro 
+ (begin
+    intro h, unfold omap at h, 
+    cases (dest_option (f a)) with ho ho, 
+    rewrite ho at h, 
+    cases (exp_mem_omap^.elim_left h) with a' ha', 
+    cases ha' with ha1' ha2',
+    existsi a', apply and.intro (or.inr ha1') ha2',
+    cases ho with b' hb', rewrite hb' at h,
+    unfold omap at h, rewrite mem_cons_iff at h,
+    cases h with h h, existsi a,
+    apply and.intro (or.inl rfl), rewrite h,
+    apply eq.symm hb',
+    cases (exp_mem_omap^.elim_left h) with a' ha', 
+    cases ha' with ha1' ha2',
+    existsi a', apply and.intro (or.inr ha1') ha2'
+  end)
+ (begin 
+   intro h, cases h with a' ha', 
+   cases ha' with h1 h2, rewrite mem_cons_iff at h1, 
+   cases h1 with h1 h1, 
+   unfold omap, subst h1, rewrite eq.symm h2, 
+   apply or.inl rfl, apply mem_omap_of_mem_omap_tail,
+   apply exp_mem_omap^.elim_right, existsi a',
+   apply and.intro h1 h2
+  end)
+  
 
 lemma exists_maximum [linear_order β] : 
 ∀ (bs : list β) (hi : bs ≠ []), ∃ b, b ∈ bs ∧ ∀ b' ∈ bs, b' ≤ b 
@@ -185,12 +209,12 @@ lemma exists_maximum [linear_order β] :
     apply @classical.by_cases (b ≤ bm); intro hle,
 
     existsi bm, apply and.intro (or.inr hbm1), 
-    intros bl hbl, rewrite exp_mem_cons at hbl, 
+    intros bl hbl, rewrite mem_cons_iff at hbl, 
     cases hbl with hbl hbl, subst hbl, apply hle, 
     apply hbm2 _ hbl,
 
     existsi b, apply and.intro (or.inl rfl),
-    intros bl hbl, rewrite exp_mem_cons at hbl, 
+    intros bl hbl, rewrite mem_cons_iff at hbl, 
     cases hbl with hbl hbl, subst hbl, 
     apply le_trans, apply hbm2 _ hbl, 
     apply le_of_not_le hle, 
@@ -201,294 +225,181 @@ lemma exists_minimum [hlo : linear_order β] :
 ∀ (bs : list β) (hi : bs ≠ []), ∃ b, b ∈ bs ∧ ∀ b' ∈ bs, b' ≥ b :=  
 @exists_maximum _ (converse_linear_order hlo)
 
-lemma mem_omap {f : α → option β} {a} {b} (he : f a = some b) : 
-  ∀ {as : list α} (HM : a ∈ as), b ∈ list.omap f as  
-| [] hm := by cases hm
-| (a'::as) hm :=
-  begin 
-    unfold has_mem.mem at hm, unfold list.mem at hm,
-    cases hm with hm hm, subst hm,
-    unfold list.omap, rewrite he, apply or.inl rfl,
-    unfold list.omap, cases (f a'), 
-    apply mem_omap, apply hm, 
-    apply or.inr, apply mem_omap, apply hm 
-  end 
-
-lemma mem_omap_of_mem_omap_tail {f : α → option β} {a} {b} :
-  ∀ {as : list α}, b ∈ list.omap f as → b ∈ list.omap f (a::as) := 
-begin
-  intros as h, unfold list.omap, cases (f a),
-  apply h, apply or.inr h
-end
 
 lemma dest_list : ∀ (as : list α), as = [] ∨ ∃ a' as', as = (a'::as')
 | [] := or.inl rfl 
 | (a::as) := begin apply or.inr, existsi a, existsi as, refl end
 
-lemma exp_mem_omap {f : α → option β} {b : β} : ∀ {as : list α}, (b ∈ list.omap f as) ↔ ∃ a, a ∈ as ∧ some b = f a 
-| [] := 
-  iff.intro 
-    (by {intro h, cases h}) 
-    (begin intro h, cases h with a ha, cases ha^.elim_left end)
-| (a::as) := 
- iff.intro 
- (begin
-    intro h, unfold list.omap at h, 
-    cases (dest_option (f a)) with ho ho, 
-    rewrite ho at h, 
-    cases (exp_mem_omap^.elim_left h) with a' ha', 
-    cases ha' with ha1' ha2',
-    existsi a', apply and.intro (or.inr ha1') ha2',
-    cases ho with b' hb', rewrite hb' at h,
-    unfold list.omap at h, rewrite exp_mem_cons at h,
-    cases h with h h, existsi a,
-    apply and.intro (or.inl rfl), rewrite h,
-    apply eq.symm hb',
-    cases (exp_mem_omap^.elim_left h) with a' ha', 
-    cases ha' with ha1' ha2',
-    existsi a', apply and.intro (or.inr ha1') ha2'
-  end)
- (begin 
-   intro h, cases h with a' ha', 
-   cases ha' with h1 h2, rewrite exp_mem_cons at h1, 
-   cases h1 with h1 h1, 
-   unfold list.omap, subst h1, rewrite eq.symm h2, 
-   apply or.inl rfl, apply mem_omap_of_mem_omap_tail,
-   apply exp_mem_omap^.elim_right, existsi a',
-   apply and.intro h1 h2
-  end)
 
-def list.product : list α → list β → list (α × β) 
-| [] _ := []
-| (a1::l1) l2 := (list.map (λ a2, ⟨a1,a2⟩) l2) ++ list.product l1 l2 
+-- def list.product : list α → list β → list (α × β) 
+-- | [] _ := []
+-- | (a1::l1) l2 := (list.map (λ a2, ⟨a1,a2⟩) l2) ++ list.product l1 l2 
 
-lemma product_nil : ∀ {l : list α}, list.product l (@list.nil β) = [] 
-| [] := by unfold list.product   
-| (a::as) := 
-  begin unfold list.product, rewrite product_nil, simp, end
-
-def list.first (p : α → Prop) [decidable_pred p] : list α → option (α × list α)
+def pluck (p : α → Prop) [decidable_pred p] : list α → option (α × list α)
 | []      := none 
 | (a::as) := 
   if p a 
   then some (a, as) 
-  else do (a',as') ← list.first as, 
+  else do (a',as') ← pluck as, 
           some (a',a::as')
 
-def exp_mem_insert [hd : decidable_eq α] {a1 a2 : α} {as : list α} :
-  a1 ∈ (list.insert a2 as) ↔ (a1 = a2 ∨ a1 ∈ as) := 
+def pluck_true (p : α → Prop) [decidable_pred p] (a as) (ha : p a) :
+  pluck p (a::as) = some (a,as) := 
+begin unfold pluck, rewrite ite_true, apply ha end
+
+def pluck_false (p : α → Prop) [decidable_pred p] (a as) (ha : ¬ p a) :
+  pluck p (a::as) 
+  = (do (a',as') ← pluck p as, some (a',a::as') ) := 
+begin unfold pluck, rewrite ite_false, refl, apply ha end
+
+/- equiv -/
+
+def equiv (l1 l2 : list α) := l1 ⊆ l2 ∧ l2 ⊆ l1
+
+notation l1 `≃` l2 := equiv l1 l2
+
+def equiv.refl {l : list α} : l ≃ l := 
+and.intro (subset.refl _) (subset.refl _)
+
+lemma equiv.trans {l1 l2 l3 : list α} : (l1 ≃ l2) → (l2 ≃ l3) → (l1 ≃ l3) :=  
 begin
-  unfold list.insert,  
-  apply @cases_ite _ (a2 ∈ as) 
-    (λ as', a1 ∈ as' ↔ a1 = a2 ∨ a1 ∈ as)
-    _ as _; intro h1; apply iff.intro; intro h2,
-  apply or.inr h2,
-  cases h2 with h2 h2, subst h2, apply h1, apply h2,
-  rewrite exp_mem_cons at h2, apply h2,    
-  rewrite exp_mem_cons, apply h2 
-end
-
-meta def unfold_list_union := 
-`[unfold has_union.union, unfold list.union, unfold list.foldr] 
-
-lemma exp_cons_union [decidable_eq α] (a : α) (as1 as2) : 
-  (a::as1) ∪ as2 = list.insert a (as1 ∪ as2) := rfl
-
-lemma mem_union_of_mem_left [decidable_eq α] {a : α} : 
-  ∀ {as1 as2 : list α}, (a ∈ as1) → a ∈ (as1 ∪ as2)  
-| [] as2 hm := by cases hm
-| (a1::as1) as2 hm := 
-  begin
-    rewrite exp_mem_cons at hm,
-    rewrite exp_cons_union, 
-    rewrite exp_mem_insert, 
-    cases hm with hm hm,
-    apply or.inl hm, 
-    apply or.inr (mem_union_of_mem_left hm) 
-  end
-
-lemma mem_union_of_mem_right [decidable_eq α] {a : α} : 
-  ∀ {as1 as2 : list α}, (a ∈ as2) → a ∈ (as1 ∪ as2)  
-| [] as2 hm := hm
-| (a1::as1) as2 hm := 
-  begin
-    rewrite exp_cons_union, rewrite exp_mem_insert, 
-    apply or.inr, apply mem_union_of_mem_right hm
-  end
-
-lemma mem_union_of_mem_either [decidable_eq α] {a : α}  
-  {as1 as2 : list α} (h : a ∈ as1 ∨ a ∈ as2) : a ∈ (as1 ∪ as2) := 
-begin
-  cases h with h h, 
-  apply mem_union_of_mem_left h, 
-  apply mem_union_of_mem_right h 
-end
-
-lemma mem_either_of_mem_union [decidable_eq α] {a : α} : 
-  ∀ {as1 as2 : list α} (hm : a ∈ (as1 ∪ as2)), a ∈ as1 ∨ a ∈ as2 
-| [] as2 hm := or.inr hm  
-| (a1::as1) as2 hm := 
-  begin
-    rewrite exp_cons_union at hm,
-    rewrite exp_mem_insert at hm, 
-    cases hm with hm hm, 
-    apply or.inl (or.inl hm),
-    cases (mem_either_of_mem_union hm) with hm' hm',
-    apply or.inl (or.inr hm'),
-    apply or.inr hm'
-  end
-
-lemma exp_mem_union[decidable_eq α] {a : α}  {as1 as2 : list α} :
-  (a ∈ as1 ∪ as2) ↔ (a ∈ as1 ∨ a ∈ as2) := 
-  iff.intro mem_either_of_mem_union mem_union_of_mem_either
-
-def list.eqmem (l1 l2 : list α) := ∀ (a : α), (a ∈ l1 ↔ a ∈ l2)
-
-def eqmem_refl {l : list α} : list.eqmem l l := λ a, iff.refl _
-
-lemma eqmem_trans {l1 l2 l3 : list α} : list.eqmem l1 l2 → list.eqmem l2 l3 → list.eqmem l1 l3 :=  
-begin
-  intros H1 H2, intro x, apply iff.trans,
-  apply H1, apply H2
+  intros h1 h2,
+  cases h1 with h1a h1b, cases h2 with h2a h2b, 
+  apply and.intro (subset.trans h1a h2a) (subset.trans h2b h1b),
 end 
 
-lemma eqmem_swap {a1 a2 : α} {l} : list.eqmem (a1::a2::l) (a2::a1::l) :=  
+lemma subset.swap {a1 a2 : α} {l} : (a1::a2::l) ⊆ (a2::a1::l) :=  
 begin
-  intro a, apply iff.intro, 
-  intro H, cases H with H H, subst H, 
-  apply or.inr, apply or.inl, refl,
-  cases H with H H, subst H, 
-  apply or.inl, refl,
-  apply or.inr, apply or.inr, apply H,
-  intro H, cases H with H H, subst H, 
-  apply or.inr, apply or.inl, refl,
-  cases H with H H, subst H, 
-  apply or.inl, refl,
-  apply or.inr, apply or.inr, apply H,
+  intros a ha, cases ha with ha ha,
+  apply or.inr (or.inl ha), cases ha with ha ha,
+  apply or.inl ha, apply or.inr (or.inr ha)
 end
 
-lemma eqmem_cons {a : α} {l1 l2} : list.eqmem l1 l2 → list.eqmem (a::l1) (a::l2) := 
+lemma equiv.swap {a1 a2 : α} {l} : (a1::a2::l) ≃ (a2::a1::l) :=  
+begin apply and.intro; apply subset.swap end
+
+lemma cons_equiv_cons {a : α} {l1 l2} : (l1 ≃ l2) → ((a::l1) ≃ (a::l2)) := 
 begin
-  intros H a', apply iff.intro, 
-  intro HM, cases HM with HM HM, 
-  apply or.inl HM, apply or.inr, 
-  apply (H a')^.elim_left, apply HM,
-  intro HM, cases HM with HM HM, 
-  apply or.inl HM, apply or.inr, 
-  apply (H a')^.elim_right, apply HM,
+  intro h, cases h with hl hr,
+  apply and.intro; apply cons_subset_cons; assumption
 end
 
-def allp (P : α → Prop) (l : list α) := ∀ a, a ∈ l → P a
+-- def allp (P : α → Prop) (l : list α) := ∀ a, a ∈ l → P a
 
 def anyp (P : α → Prop) (l : list α) := ∃ a, a ∈ l ∧ P a
 
-lemma allp_nil {P : α → Prop} : allp P [] :=
-begin intros _ H, cases H end
+-- lemma allp_nil {P : α → Prop} : allp P [] :=
+-- begin intros _ H, cases H end
 
-lemma allp_tail_of_allp {P : α → Prop} {a as} : allp P (a::as) → allp P as :=
-begin intros h x hx, apply h, apply or.inr, apply hx end
+-- lemma allp_tail_of_allp {P : α → Prop} {a as} : allp P (a::as) → allp P as :=
+-- begin intros h x hx, apply h, apply or.inr, apply hx end
+-- ==> list.forall_mem_of_forall_mem_cons
 
-lemma allp_of_allp_cons {P : α → Prop} {a} {as} (h : allp P (a::as)) : 
-  allp P as :=
-begin intros a' ha', apply h, apply or.inr ha' end
+-- lemma allp_of_allp_cons {P : α → Prop} {a} {as} (h : allp P (a::as)) : 
+--   allp P as :=
+-- begin intros a' ha', apply h, apply or.inr ha' end
+-- ==> list.forall_mem_of_forall_mem_cons
 
+-- lemma exp_allp_nil {P : α → Prop} : allp P [] ↔ true :=
+-- true_iff_true allp_nil trivial
 
-lemma exp_allp_nil {P : α → Prop} : allp P [] ↔ true :=
-true_iff_true allp_nil trivial
+-- lemma allp_of_allp {P Q : α → Prop} (H : ∀ a, P a → Q a) 
+--   (as) (HP : allp P as) : allp Q as :=
+-- begin intros a Ha, apply H, apply HP, apply Ha end
 
-lemma allp_of_allp {P Q : α → Prop} (H : ∀ a, P a → Q a) 
-  (as) (HP : allp P as) : allp Q as :=
-begin intros a Ha, apply H, apply HP, apply Ha end
+-- lemma allp_union_of_allp_both [decidable_eq α] {P : α → Prop} {as1 as2}  
+--   (h : allp P as1 ∧ allp P as2) : allp P (as1 ∪ as2) :=
+-- begin
+--   cases h with h1 h2, intros a ha, 
+--   rewrite mem_union at ha, 
+--   cases ha with ha ha, 
+--   apply h1 _ ha, apply h2 _ ha,
+-- end
 
-lemma allp_union_of_allp_both [decidable_eq α] {P : α → Prop} {as1 as2}  
-  (h : allp P as1 ∧ allp P as2) : allp P (as1 ∪ as2) :=
-begin
-  cases h with h1 h2, intros a ha, 
-  rewrite exp_mem_union at ha, 
-  cases ha with ha ha, 
-  apply h1 _ ha, apply h2 _ ha,
-end
+-- lemma allp_both_of_allp_union [decidable_eq α] {P : α → Prop} {as1 as2}  
+--   (h : allp P (as1 ∪ as2)) : allp P as1 ∧ allp P as2 :=
+-- begin
+--   apply and.intro; intros a ha; apply h,
+--   apply mem_union_left ha,
+--   apply mem_union_right ha
+-- end
+-- 
+-- lemma exp_allp_union [decidable_eq α] (P : α → Prop) (as1 as2) :
+--   (allp P (as1 ∪ as2)) ↔ (allp P as1 ∧ allp P as2) :=
+-- iff.intro allp_both_of_allp_union allp_union_of_allp_both
+-- 
+-- def dec_allp {P : α → Prop} [HP : decidable_pred P] : decidable_pred (allp P)  
+-- | [] := is_true (by apply allp_nil)
+-- | (a::as) := 
+--   begin
+--     cases (HP a) with HP HP, apply is_false, intro HC,  
+--     apply absurd (HC a (or.inl (by refl))) HP,
+--     cases (dec_allp as) with Has Has, 
+--     apply is_false, intro HC, apply Has, 
+--     intros x Hx, apply HC, apply or.inr Hx, 
+--     apply is_true, intros x Hx, cases Hx with Hx Hx,
+--     rewrite Hx, apply HP, apply Has x Hx 
+--   end
 
-lemma allp_both_of_allp_union [decidable_eq α] {P : α → Prop} {as1 as2}  
-  (h : allp P (as1 ∪ as2)) : allp P as1 ∧ allp P as2 :=
-begin
-  apply and.intro; intros a ha; apply h,
-  apply mem_union_of_mem_left ha,
-  apply mem_union_of_mem_right ha
-end
-
-lemma exp_allp_union [decidable_eq α] (P : α → Prop) (as1 as2) :
-  (allp P (as1 ∪ as2)) ↔ (allp P as1 ∧ allp P as2) :=
-iff.intro allp_both_of_allp_union allp_union_of_allp_both
-
-def dec_allp {P : α → Prop} [HP : decidable_pred P] : decidable_pred (allp P)  
-| [] := is_true (by apply allp_nil)
-| (a::as) := 
-  begin
-    cases (HP a) with HP HP, apply is_false, intro HC,  
-    apply absurd (HC a (or.inl (by refl))) HP,
-    cases (dec_allp as) with Has Has, 
-    apply is_false, intro HC, apply Has, 
-    intros x Hx, apply HC, apply or.inr Hx, 
-    apply is_true, intros x Hx, cases Hx with Hx Hx,
-    rewrite Hx, apply HP, apply Has x Hx 
-  end
-
-
-lemma cases_first (P : α → Prop) [HD : decidable_pred P] : ∀ (as : list α), 
-(list.first P as = none ∧ allp (λ x, ¬ P x) as) 
-∨ ∃ (a) (as'), (list.first P as = some (a,as') ∧ P a ∧ list.eqmem as (a::as'))
+lemma cases_pluck (P : α → Prop) [hd : decidable_pred P] : ∀ (as : list α), 
+(pluck P as = none ∧ (∀ x ∈ as, ¬ P x)) 
+∨ ∃ (a) (as'), (pluck P as = some (a,as') ∧ P a ∧ (as ≃ (a::as')))
 | [] := 
   begin 
     apply or.inl, apply and.intro, 
-    unfold list.first, intros _ H, cases H
+    unfold pluck, intros _ H, cases H
   end
 | (a::as) :=
   begin
-    repeat {unfold list.first, unfold ite}, simp,
-    cases (HD a) with Ha Ha, simp, 
-    cases (cases_first as) with Has Has,  
-    cases Has with Has1 Has2, 
-    apply or.inl, apply and.intro, 
-    intros x Hx, cases Hx with Hx Hx,
-    rewrite Hx, apply Ha, apply Has2, apply Hx,
-    rewrite Has1, refl, 
-    cases Has with x Has, cases Has with xs Hx,  
-    apply or.inr, existsi x, existsi (a::xs),
-    cases Hx with Hx1 Hx, cases Hx with Hx2 Hx3, 
-    apply and.intro, apply Hx2, 
-    apply and.intro, 
-    apply eqmem_trans _ eqmem_swap,
-    apply eqmem_cons Hx3, rewrite Hx1,
-    refl, apply or.inr, existsi a, existsi as,
-    apply and.intro Ha, apply and.intro, 
-    apply eqmem_refl, simp
+    cases (hd a) with ha ha, 
+    cases (cases_pluck as) with has has,
+
+    apply or.inl, cases has with has1 has2,
+    apply and.intro, rewrite pluck_false,
+    rewrite has1, refl, apply ha,
+    rewrite forall_mem_cons,
+    apply and.intro ha has2,
+
+    apply or.inr, cases has with a' has,
+    cases has with as' has',
+    cases has' with h1 has', cases has' with h2 h3,
+    existsi a', existsi (a::as'),
+    apply and.intro, rewrite pluck_false, 
+    rewrite h1, refl, apply ha, apply and.intro h2,
+    apply equiv.trans, apply cons_equiv_cons, 
+    apply h3, apply equiv.swap,
+    
+    apply or.inr, existsi a, existsi as,
+    apply and.intro, rewrite pluck_true, apply ha,
+    apply and.intro ha equiv.refl
   end
 
-@[simp] def list.nth_dft (a : α) (l : list α) (n : nat) : α :=  
-match list.nth l n with 
+
+
+@[simp] def nth_dft (a : α) (l : list α) (n : nat) : α :=  
+match nth l n with 
 | none := a 
 | (some a') := a'
 end
 
-def list.head_dft (a' : α) : list α → α 
+def head_dft (a' : α) : list α → α 
 | [] := a'
 | (a::as) := a 
 
 lemma nth_pred (a : α) (l : list α) (n : nat) (H : n > 0) : 
-list.nth (a::l) n = list.nth l (n - 1) := 
+nth (a::l) n = nth l (n - 1) := 
 begin cases n, cases H, simp end
 
 lemma nth_dft_pred {a a' : α} {l : list α} {n : nat} (H : n > 0) : 
-list.nth_dft a (a'::l) n = list.nth_dft a l (n - 1) :=
-begin unfold list.nth_dft, rewrite nth_pred, apply H  end
+nth_dft a (a'::l) n = nth_dft a l (n - 1) :=
+begin unfold nth_dft, rewrite nth_pred, apply H  end
 
 lemma nth_dft_succ {a a' : α} {l : list α} {n : nat} : 
-list.nth_dft a (a'::l) (n+1) = list.nth_dft a l n :=
-begin unfold list.nth_dft, simp  end
+nth_dft a (a'::l) (n+1) = nth_dft a l n :=
+begin unfold nth_dft, simp  end
 
-lemma nth_dft_head {a a' : α} {as : list α} : list.nth_dft a' (a::as) 0 = a := 
-begin unfold list.nth_dft, simp end
+lemma nth_dft_head {a a' : α} {as : list α} : nth_dft a' (a::as) 0 = a := 
+begin unfold nth_dft, simp end
 
 def append_pair {α : Type} : (list α × list α) → list α  
 | (l1,l2) := l1 ++ l2 
@@ -516,7 +427,7 @@ lemma some_true_iff_disj_list :
   begin
     unfold some_true, unfold disj_list, 
     apply iff.intro; intro h, cases h with x hx,
-    cases hx with hx1 hx2, rewrite exp_mem_cons at hx1,
+    cases hx with hx1 hx2, rewrite mem_cons_iff at hx1,
     cases hx1 with hx1 hx1, subst hx1, apply or.inl hx2, 
     rewrite iff.symm some_true_iff_disj_list,
     apply or.inr, existsi x, apply and.intro hx1 hx2,
@@ -598,126 +509,73 @@ begin
   apply or.inr, apply Hl, apply Hr 
 end
 
-def ex_arg_of_mem_map {f : α → β} {b : β} : 
-  ∀ {as : list α}, (b ∈ list.map f as) → ∃ a, a ∈ as ∧ b = f a 
-| [] H := by cases H 
-| (a::as) H := 
-  begin
-    simp at H, cases H with H H, existsi a, 
-    apply and.intro (or.inl (eq.refl _)) H,  
-    cases (ex_arg_of_mem_map H) with a' Ha',
-    existsi a', apply and.intro, 
-    apply or.inr (Ha'^.elim_left), 
-    apply Ha'^.elim_right
-  end
+
+-- def ex_arg_of_mem_map {f : α → β} {b : β} : 
+--   ∀ {as : list α}, (b ∈ list.map f as) → ∃ a, a ∈ as ∧ b = f a 
+-- | [] H := by cases H 
+-- | (a::as) H := 
+--   begin
+--     simp at H, cases H with H H, existsi a, 
+--     apply and.intro (or.inl (eq.refl _)) H,  
+--     cases (list.exists_of_mem_map H) with a' Ha',
+--     existsi a', apply and.intro, 
+--     apply or.inr (Ha'^.elim_left), 
+--     apply Ha'^.elim_right
+--   end
+
 
 lemma fst_mem_of_mem_product : 
   ∀ {as : list α} {bs : list β} {p : α × β}, 
-    p ∈ (list.product as bs) → (prod.fst p) ∈ as  
-| [] bs b H := begin unfold list.product at H, cases H end
-| (a::as) bs b H := 
+    p ∈ (product as bs) → (prod.fst p) ∈ as  
+| [] bs b H := begin unfold product at H, cases H end
+| (a::as) bs ab h := 
   begin
-    unfold list.product at H, simp at H, cases H with H H,
-    apply or.inr, apply fst_mem_of_mem_product, apply H,
-    cases (ex_arg_of_mem_map H) with x Hx, 
-    rewrite Hx^.elim_right, apply or.inl, refl
+    unfold product at h, simp at h, cases h with h h,
+    
+    cases h with b hb, cases hb with hb1 hb2,
+    rewrite eq.symm hb2, apply or.inl rfl, 
+
+    cases h with a' h, cases h with h1 h2, 
+    cases h2 with b hb, cases hb with hb1 hb2, 
+    rewrite eq.symm hb2, apply or.inr, apply h1
   end
 
 lemma snd_mem_of_mem_product : 
   ∀ {as : list α} {bs : list β} {p : α × β}, 
-    p ∈ (list.product as bs) → (prod.snd p) ∈ bs 
-| [] bs b H := begin unfold list.product at H, cases H end
-| (a::as) bs b H := 
+    p ∈ (product as bs) → (prod.snd p) ∈ bs 
+| [] bs b H := begin unfold product at H, cases H end
+| (a::as) bs ab h := 
   begin
-    unfold list.product at H, simp at H, cases H with H H,
-    apply snd_mem_of_mem_product, apply H,
-    cases (ex_arg_of_mem_map H) with x Hx, 
-    rewrite Hx^.elim_right, apply Hx^.elim_left
+    unfold product at h, simp at h, cases h with h h,
+    
+    cases h with b hb, cases hb with hb1 hb2,
+    rewrite eq.symm hb2, apply hb1, 
+
+    cases h with a' h, cases h with h1 h2, 
+    cases h2 with b hb, cases hb with hb1 hb2, 
+    rewrite eq.symm hb2, apply hb1
   end
 
-def mem_map_of_mem {f : α → β} : ∀ {as : list α} {a : α}, a ∈ as → (f a) ∈ list.map f as 
-| [] a H := by cases H 
-| (a'::as) a H := 
-  begin
-    unfold list.map, cases H with H H,
-    rewrite H, apply or.inl (eq.refl _),
-    apply or.inr, apply @mem_map_of_mem as a H
-  end
 
-def mem_map_of_ex_arg {f : α → β} {b : β} : 
-  ∀ {as : list α}, (∃ a, a ∈ as ∧ b = f a) → b ∈ list.map f as := 
-begin
-  intros as hex, cases hex with a ha,
-  cases ha with ha1 ha2, subst ha2,
-  apply mem_map_of_mem ha1,
-end
-
-def exp_mem_map {f : α → β} {b : β} {as : list α} : 
- (b ∈ list.map f as) ↔ (∃ a, a ∈ as ∧ b = f a) :=
-iff.intro (ex_arg_of_mem_map) (mem_map_of_ex_arg)
-
-lemma allp_map (P : α → Prop) {Q : β → Prop} {f : α → β} {as} : 
-allp P as → (∀ a, P a → Q (f a)) → allp Q (list.map f as) := 
+lemma forall_mem_map_of_forall_mem (P : α → Prop) {Q : β → Prop} {f : α → β} {as} : 
+(∀ a ∈ as, P a) → (∀ a, P a → Q (f a)) → (∀ b ∈ (map f as), Q b) := 
 begin
   intros has hf b hb, 
-  rewrite exp_mem_map at hb, 
+  rewrite mem_map at hb, 
   cases hb with a ha, cases ha with ha1 ha2,
   subst ha2, apply hf, apply has, apply ha1
 end
 
-lemma mem_product_of_mem_of_mem :
-  ∀ {as : list α} {bs : list β} {a : α} {b : β}, 
-    a ∈ as → b ∈ bs → (a,b) ∈ list.product as bs 
-| [] _ _ _ H _ := by cases H
-| _ [] _ _ _ H := by cases H
-| (a::as) (b::bs) a' b' Ha Hb := 
-  begin
-    unfold has_mem.mem at Ha, unfold list.mem at Ha, 
-    unfold has_mem.mem at Hb, unfold list.mem at Hb, 
-    unfold has_mem.mem, unfold list.product, unfold list.map, 
-    unfold append, simp, unfold list.mem,
-    cases Ha with Ha Ha, cases Hb with Hb Hb, 
-    apply or.inl, simp *, 
-    apply or.inr, apply mem_append_of_mem_or_mem,
-    apply or.inl, simp *, apply mem_map_of_mem, 
-    apply Hb, apply or.inr, apply mem_append_of_mem_or_mem,
-    apply or.inr, apply mem_product_of_mem_of_mem,
-    apply Ha, apply Hb
-  end
+lemma mem_product_of_mem_and_mem {as : list α} {bs : list β} 
+  {a : α} {b : β} (h : a ∈ as ∧ b ∈ bs) : (a,b) ∈ product as bs := 
+begin rewrite mem_product, apply h end
 
-lemma map_dist_append {f : α → β} : 
-  ∀ (l1 l2 : list α), list.map f (l1 ++ l2) = (list.map f l1) ++ (list.map f l2) := 
-begin
-  intro l1, induction l1, intro l2, simp *,
-  intro l2, rename a_1 l1,
-  repeat {unfold append, unfold list.append}, 
-  repeat {unfold list.map}, unfold list.append,
-  apply congr_arg (list.cons (f a)), apply ih_1
-end
 
-def mem_filter_of_pred_and_mem {P : α → Prop} [HD : decidable_pred P] : 
-  ∀ (as : list α) (a : α), P a → a ∈ as → a ∈ list.filter P as 
-| [] a HP HM := by cases HM 
-| (a'::as) a HP HM := 
-  begin
-    unfold list.filter, unfold ite, 
-    unfold has_mem.mem at HM, unfold list.mem at HM,
-    cases HM with HM HM, 
-    cases (HD a') with HD HD, 
-    exfalso, apply HD, rewrite HM at HP, apply HP,
-    simp, apply or.inl HM,  
-    cases (HD a') with HD HD, simp, 
-    apply mem_filter_of_pred_and_mem, apply HP, 
-    apply HM, simp, 
-    apply or.inr, apply mem_filter_of_pred_and_mem,
-    apply HP, apply HM
-  end
-
-lemma map_eq (f g : α → β)  : ∀ (as : list α) (H : ∀ a, a ∈ as → f a = g a), list.map f as = list.map g as 
+lemma map_eq (f g : α → β) : ∀ (as : list α) (H : ∀ a ∈ as, f a = g a), map f as = map g as 
 | [] _ := eq.refl _
 | (a::as) H := 
   begin 
-    unfold list.map, rewrite H, rewrite map_eq,
+    unfold map, rewrite H, rewrite map_eq,
     intros a Ha, apply (H _ (or.inr Ha)),  
     apply (or.inl (eq.refl _))
   end
@@ -726,47 +584,27 @@ meta def first_arg (f : α → tactic β) : list α → tactic β
 | [] := tactic.failed 
 | (a::as) := f a <|> (first_arg as)
 
-lemma eq_of_mem_singleton {a a' : α} : a ∈ [a'] → a = a' :=
-begin unfold has_mem.mem, unfold list.mem, rewrite or_false, apply id end
-
-lemma mem_of_mem_filter {P : α → Prop} {a : α} : 
-  ∀ {l : list α} {HD : decidable_pred P}, a ∈ (@list.filter _ P HD l) → a ∈ l  
-| [] _ := by {intro H, cases H} 
-| (a'::as) HD := 
-  begin
-    unfold list.filter, unfold ite, 
-    cases (HD a') with HD HD, simp, intro HM, 
-    apply or.inr, apply mem_of_mem_filter HM,
-    simp, intro HM, cases HM with H1 H2, 
-    apply or.inl H1, apply or.inr, 
-    apply mem_of_mem_filter H2,
-  end 
-
-lemma allp_filter_cond (P : α → Prop) [H : decidable_pred P] : ∀ (l : list α) , allp P (list.filter P l) 
-| [] := begin intros _ Ha, cases Ha end 
-| (x::xs) := 
-  begin 
-    unfold list.filter, unfold ite, 
-    cases (H x) with H1 H1, simp, apply allp_filter_cond, 
-    simp, intros a Ha, cases Ha with H2 H3, rewrite H2,
-    apply H1, apply allp_filter_cond, apply H3
-  end
-
-lemma allp_filter_of_allp {P Q : α → Prop} [H : decidable_pred Q] 
-  {as : list α} (h : allp P as) : allp P (list.filter Q as) := 
+-- lemma allp_filter_cond (P : α → Prop) [H : decidable_pred P] : ∀ (l : list α) , allp P (list.filter P l) 
+-- | [] := begin intros _ Ha, cases Ha end 
+-- | (x::xs) := 
+--   begin 
+--     unfold list.filter, unfold ite, 
+--     cases (H x) with H1 H1, simp, apply allp_filter_cond, 
+--     simp, intros a Ha, cases Ha with H2 H3, rewrite H2,
+--     apply H1, apply allp_filter_cond, apply H3
+--   end
+-- 
+lemma forall_mem_filter_of_forall_mem {P Q : α → Prop} [H : decidable_pred Q] 
+  {as : list α} (h : ∀ a ∈ as, P a) : ∀ a ∈ (list.filter Q as), P a := 
 begin
   intros a ha, apply h, 
   apply mem_of_mem_filter ha 
 end
 
-lemma pred_of_mem_filter_pred {P : α → Prop} {a : α} : 
-  ∀ {l : list α} {HD : decidable_pred P}, a ∈ (@list.filter _ P HD l) → P a 
-| [] HD := by {intro H, cases H} 
-| (a'::as) HD := 
-  begin
-    unfold list.filter, unfold ite, 
-    cases (HD a') with HD HD, simp, 
-    intro Ha, apply pred_of_mem_filter_pred, apply Ha,
-    intro Ha, cases Ha with Ha Ha, rewrite Ha, apply HD,
-    apply pred_of_mem_filter_pred, apply Ha
-  end 
+@[simp] def allp (P : α → Prop) (as : list α) := ∀ a ∈ as, P a
+
+lemma allp_iff_forall_mem (P : α → Prop) (as : list α) :
+  (allp P as) ↔ (∀ a ∈ as, P a) :=
+by unfold allp
+
+end list
