common/predicates.lean
@@ -2,10 +2,10 @@ import .atom
 
 variables {α β : Type}
 
-def qfree_prsv (qe : fm α → fm α) := 
+def qfree_of_nqfree (qe : fm α → fm α) := 
 ∀ (p : fm α), nqfree p → qfree (qe p)
 
-def normal_prsv (β) [atom_type α β] (qe : fm α → fm α) := 
+def qfree_of_fnormal_of_nqfree (β) [atom_type α β] (qe : fm α → fm α) := 
 ∀ (p : fm α), nqfree p → fnormal β p → qfree (qe p)
 
 def interp_prsv_ex (β) [atom_type α β] (qe : fm α → fm α) (p) := 
