common/test.lean
@@ -1,0 +1,9 @@
+import ...mathlib.data.int.basic
+
+set_option class.instance_max_depth 256
+
+namespace int 
+
+def foobar (i j : int) : Prop := (has_dvd.dvd i j)
+
+end int
